changed to parameterized, now verifies quickly

GenericCountingSort.dfy
@@ -67,45 +67,52 @@ ensures(filter(filter(a, f), g) == filter(a, y => f(y) && g(y))) {
 
 }
 
+
+//Everything is parametric in the type G and function key (from mergesort example)
+type G
+
+function method key(x : G) : int
+
 //Proofs about filtering lists by lt/leq/eq relations
 
-lemma {:induction a} filter_lt_decompose<T>(a: seq<T>, b : int, key : T -> int)
+lemma {:induction a} filter_lt_decompose(a: seq<G>, b : int)
 ensures(|filter(a, y => key(y) < b)| == |filter(a, y => key(y) < b - 1)| + |filter(a, y => key(y) == b - 1)|) {
 }
 
-lemma {:induction a} filter_leq_decompose<T>(a: seq<T>, x : int, key : T -> int)
+lemma {:induction a} filter_leq_decompose(a: seq<G>, x : int)
 ensures(|filter(a, y => key(y) <= x)| == |filter(a, y => key(y) < x)| + |filter(a, y => key(y) == x)|) {
 }
 
-lemma filter_lt_leq_minus_one<T>(a: seq<T>, x : int, key : T -> int)
+lemma filter_lt_leq_minus_one(a: seq<G>, x : int)
 ensures(filter(a, y => key(y) < x) == filter(a, y => key(y) <= x - 1)) {
 }
 
 //NOTE
-lemma {:induction a} filter_bounded_in<T>(a:seq<T>, x : int, y : int, key : T -> int)
+lemma {:induction a} filter_bounded_in(a:seq<G>, x : int, y : int)
 requires(x < y)
 requires(exists t  :: t in a && key(t) == y)
 ensures(|filter(a, z => x < key(z) && key(z) <= y)| > 0){
 }
 
-lemma {: induction a} filter_leq_decompose_bounds<T>(a : seq<T>, x : int, y : int, key : T -> int)
+lemma {: induction a} filter_leq_decompose_bounds(a : seq<G>, x : int, y : int)
 requires (x <= y)
 ensures (|filter(a, z => key(z) <= y)| == |filter(a, z => key(z) <= x)| + |filter(a, z => x < key(z) && key(z) <= y)|) {
 }
 
+
 // The [numLt] and [numLeq] predicates - specifies the number of elements whose key is less than/leq the given value in an array
 //  used to specify the correct position of the element in a sorted array 
 
-function numLt<T>(x: int, a : seq<T>, key : T -> int) : int {
+function numLt(x: int, a : seq<G>) : int {
   |filter(a, y => key(y) < x)|
 }
 
-function numEq<T>(x: int, a : seq<T>, key : T -> int) : int {
+function numEq(x: int, a : seq<G>) : int {
   |filter(a, y => key(y) == x)|
 }
 
-function numLeq<T>(x: int, a : seq<T>, key : T -> int) : int {
-  numLt(x, a, key) + numEq(x, a, key)
+function numLeq(x: int, a : seq<G>) : int {
+  numLt(x, a) + numEq(x, a)
 }
 
 //An element's position in the sorted array is as follows
@@ -117,65 +124,65 @@ function seqArr<T>(x: int, a : seq<T>) : seq<T> {
 
 //in reality, x = a[i] (for anything useful here)
 //NOTE: have as position of a given key - NOT an element
-function position<T>(x : int, i : int, a : seq<T>, key : T -> int) : int {
-    numLt(x, a, key) + numEq(x, seqArr(i+1, a), key) - 1
+function position(x : int, i : int, a : seq<G>) : int {
+    numLt(x, a) + numEq(x, seqArr(i+1, a)) - 1
 }
 
 //Dafny cannot infer this automatically and cannot even infer from generic versions
 //(parameterized by x) - this is a very annoying limitation
-lemma numLt_unfold_zero<T>(a : seq<T>, key : T -> int) 
-ensures(numLt(0, a, key) == |filter(a, y => key(y) < 0)|) {}
+lemma numLt_unfold_zero(a : seq<G>) 
+ensures(numLt(0, a) == |filter(a, y => key(y) < 0)|) {}
 
-lemma numEq_minus_one<T>(x: int, a : seq<T>, key : T -> int)
-ensures(numEq(x-1, a, key) == |filter(a, y => key(y) == x-1)|) {
+lemma numEq_minus_one(x: int, a : seq<G>)
+ensures(numEq(x-1, a) == |filter(a, y => key(y) == x-1)|) {
 }
 
-lemma numLt_minus_one<T>(x: int, a : seq<T>, key : T -> int)
-ensures(numLt(x-1, a, key) == |filter(a, y => key(y) < x-1)|) {
+lemma numLt_minus_one(x: int, a : seq<G>)
+ensures(numLt(x-1, a) == |filter(a, y => key(y) < x-1)|) {
 }
 
 //Some alternate characterizations that make some things easier
-lemma numLeq_direct<T>(x:int, a : seq<T>, key : T -> int) 
-ensures(numLeq(x, a, key) == |filter(a, y => key(y) <= x)|) {
+lemma numLeq_direct(x:int, a : seq<G>) 
+ensures(numLeq(x, a) == |filter(a, y => key(y) <= x)|) {
 }
 
-lemma {: induction x} numLt_ind<T>(x: int, a : seq<T>, key : T -> int)
-ensures(numLt(x, a, key) == numEq(x-1, a, key) + numLt(x-1, a, key)) {
-  numEq_minus_one(x, a, key);
-  numLt_minus_one(x, a, key);
-  filter_lt_decompose(a, x, key);
+lemma {: induction x} numLt_ind(x: int, a : seq<G>)
+ensures(numLt(x, a) == numEq(x-1, a) + numLt(x-1, a)) {
+  numEq_minus_one(x, a);
+  numLt_minus_one(x, a);
+  filter_lt_decompose(a, x);
 }
 
-lemma numLt_leq_minus_one<T>(x: int, a : seq<T>, key : T -> int)
-ensures(numLt(x, a, key) == numLeq(x-1, a, key)) {
-  numLt_ind(x, a, key);
+lemma numLt_leq_minus_one(x: int, a : seq<G>)
+ensures(numLt(x, a) == numLeq(x-1, a)) {
+  numLt_ind(x, a);
 }
 
-lemma numLeq_ind<T>(x: int, a : seq<T>, key : T -> int) 
-ensures(numLeq(x,a, key) == numLeq(x-1, a, key) + numEq(x, a, key)) {
-  numLeq_direct(x, a, key);
-  assert(numLeq(x,a, key) == |filter(a, y => key(y) <= x)|);
-  filter_leq_decompose(a, x, key);
-  numLt_leq_minus_one(x, a, key);  
+lemma numLeq_ind(x: int, a : seq<G>) 
+ensures(numLeq(x,a) == numLeq(x-1, a) + numEq(x, a)) {
+  numLeq_direct(x, a);
+  assert(numLeq(x,a) == |filter(a, y => key(y) <= x)|);
+  filter_leq_decompose(a, x);
+  numLt_leq_minus_one(x, a);  
 }
 
-lemma numEq_app<T>(x: int, a : seq<T>, b : seq<T>, key : T -> int)
-ensures(numEq(x, a + b, key) == numEq(x, a, key) + numEq(x,b, key)) {
+lemma numEq_app(x: int, a : seq<G>, b : seq<G>)
+ensures(numEq(x, a + b) == numEq(x, a) + numEq(x,b)) {
   filter_app(a, b, y => key(y) == x);
 }
 
 //NOTE
-lemma numEq_singleton<T>(x: T, y : int, key : T -> int)
+lemma numEq_singleton(x: G, y : int)
 requires(key(x) == y)
-ensures(numEq(y, [x], key) == 1) {
+ensures(numEq(y, [x]) == 1) {
   filterAll([x], z => key(z) == y);
 }
 
 
 //sorta note
-lemma {:induction a} numEq_in_pos<T>(x: T, a : seq<T>, key : T -> int)
+lemma {:induction a} numEq_in_pos(x: G, a : seq<G>)
 requires (x in a)
-ensures (numEq(key(x), a, key) > 0) {
+ensures (numEq(key(x), a) > 0) {
   if(|a| <= 0) {}
   else {
     if(a[0] == x) {
@@ -189,96 +196,96 @@ ensures (numEq(key(x), a, key) > 0) {
 // Transitivity and injectivity of [numLeq] - used in proving that counting sort does not repeat elts and 
 //  that the result is actually sorted 
 
-lemma numLeq_lt_trans<T>(a:seq<T>, x: T, y: T, key : T -> int)
+lemma numLeq_lt_trans(a:seq<G>, x: G, y: G)
 requires(key(x) < key(y))
 requires(y in a)
-ensures(numLeq(key(x), a, key) < numLeq(key(y), a, key)) {
-  numLeq_direct(key(y), a, key);
-  numLeq_direct(key(x), a, key);
-  filter_leq_decompose_bounds(a, key(x), key(y), key);
-  filter_bounded_in(a, key(x), key(y), key);
+ensures(numLeq(key(x), a) < numLeq(key(y), a)) {
+  numLeq_direct(key(y), a);
+  numLeq_direct(key(x), a);
+  filter_leq_decompose_bounds(a, key(x), key(y));
+  filter_bounded_in(a, key(x), key(y));
 }
 
 //We need 2 more similar lemmas for the sortedness equivalence proof
-lemma numLeq_leq_trans<T>(a:seq<T>, x : int, y : int, key : T -> int)
+lemma numLeq_leq_trans(a:seq<G>, x : int, y : int)
 requires(x <= y)
-ensures(numLeq(x, a, key) <= numLeq(y, a, key)) {
-    numLeq_direct(x, a, key);
-    numLeq_direct(y, a, key);
-    filter_leq_decompose_bounds(a, x, y, key);
+ensures(numLeq(x, a) <= numLeq(y, a)) {
+    numLeq_direct(x, a);
+    numLeq_direct(y, a);
+    filter_leq_decompose_bounds(a, x, y);
 }
 
-lemma numLt_leq_bound<T>(a: seq<T>, x : int, y : int, key : T -> int) 
+lemma numLt_leq_bound(a: seq<G>, x : int, y : int) 
 requires(x < y)
-ensures(numLeq(x, a, key) - 1 < numLt(y, a, key)) {
-    numLt_leq_minus_one(y, a, key);
-    numLeq_leq_trans(a, x, y-1, key);
+ensures(numLeq(x, a) - 1 < numLt(y, a)) {
+    numLt_leq_minus_one(y, a);
+    numLeq_leq_trans(a, x, y-1);
 }
 
 //what we really need - injectivity for position function - if a[i] and a[j] have the same position - i = j
 
-lemma position_bounds<T>(a: seq<T>, x: T, i : int, key : T -> int)
+lemma position_bounds(a: seq<G>, x: G, i : int)
 requires(0 <= i < |a|)
 requires(x in a[..i+1])
-ensures(numLt(key(x), a, key) <= position(key(x), i, a, key) <= numLeq(key(x), a, key) - 1) {
-  numEq_in_pos(x, a[..(i+1)], key);
-  assert(numLt(key(x), a, key) <= position(key(x), i, a, key));
+ensures(numLt(key(x), a) <= position(key(x), i, a) <= numLeq(key(x), a) - 1) {
+  numEq_in_pos(x, a[..(i+1)]);
+  assert(numLt(key(x), a) <= position(key(x), i, a));
   assert(a == a[..(i+1)] + a[(i+1)..]);
-  numEq_app(key(x), a[..(i+1)], a[(i+1)..], key);
-  assert (numEq(key(x), a[..(i+1)], key) <= numEq(key(x), a, key));
+  numEq_app(key(x), a[..(i+1)], a[(i+1)..]);
+  assert (numEq(key(x), a[..(i+1)]) <= numEq(key(x), a));
 }
 
 
-lemma position_inj<T>(a: seq<T>, i : int, j : int, key : T -> int)
+lemma position_inj(a: seq<G>, i : int, j : int)
 requires(0 <= i < |a|)
 requires(0 <= j < |a|)
-requires(position(key(a[i]), i, a, key) == position(key(a[j]), j, a, key))
+requires(position(key(a[i]), i, a) == position(key(a[j]), j, a))
 ensures(i == j) {
   //proof by contradiction
   if(i == j) {}
   else {
     if(key(a[i]) == key(a[j])) { 
-      assert(numLt(key(a[i]), a, key) == numLt(key(a[j]), a, key));
+      assert(numLt(key(a[i]), a) == numLt(key(a[j]), a));
       //both cases are similar
       if(i < j) {
         assert(a[..(j+1)] == a[..(i+1)] + a[i+1..j+1]);
-        numEq_app(key(a[j]), a[..(i+1)], a[i+1..j+1], key);
-        numEq_in_pos(a[j], a[i+1..j+1], key);
+        numEq_app(key(a[j]), a[..(i+1)], a[i+1..j+1]);
+        numEq_in_pos(a[j], a[i+1..j+1]);
       }
       else {
         assert(a[..(i+1)] == a[..(j+1)] + a[j+1..i+1]);
-        numEq_app(key(a[i]), a[..(j+1)], a[j+1..i+1], key);
-        numEq_in_pos(a[i], a[j+1..i+1], key);
+        numEq_app(key(a[i]), a[..(j+1)], a[j+1..i+1]);
+        numEq_in_pos(a[i], a[j+1..i+1]);
       }
     }
     else {
       //again, cases are similar
       if(key(a[i]) < key(a[j])) {
-        position_bounds(a, a[i], i, key);
-        position_bounds(a, a[j], j, key);
-        numLt_leq_bound(a, key(a[i]), key(a[j]), key);
+        position_bounds(a, a[i], i);
+        position_bounds(a, a[j], j);
+        numLt_leq_bound(a, key(a[i]), key(a[j]));
       }
       else {
-        position_bounds(a, a[i], i, key);
-        position_bounds(a, a[j], j, key);
-        numLt_leq_bound(a, key(a[j]), key(a[i]), key);
+        position_bounds(a, a[i], i);
+        position_bounds(a, a[j], j);
+        numLt_leq_bound(a, key(a[j]), key(a[i]));
       }
     }    
   }
 }
 
 //For equal elements, positions and indices have the same ordering
-lemma positions_eq_preserve_order<T>(a : seq<T>, k : int, i : int, x : T, key: T -> int)
+lemma positions_eq_preserve_order(a : seq<G>, k : int, i : int, x : G)
 requires(0 <= i < |a|)
 requires(0 <= k < |a|)
-requires(position(key(x), k, a[..], key) < position(key(x), i, a[..], key))
+requires(position(key(x), k, a[..]) < position(key(x), i, a[..]))
 ensures(k < i) {
   if(k < i) {
   }
   else {
     assert(i <= k);
     assert(a[..k+1] == a[..i+1] + a[i+1..k+1]);
-    numEq_app(key(x), a[..i+1], a[i+1..k+1], key);
+    numEq_app(key(x), a[..i+1], a[i+1..k+1]);
   }
 }
 
@@ -290,22 +297,22 @@ ensures(k < i) {
 
 //How position changes when we decrease index
 //NOTE
-lemma position_decr_index_same<T>(a : seq<T>, i : int, key : T -> int)
+lemma position_decr_index_same(a : seq<G>, i : int)
 requires(0 <= i < |a|)
-ensures(position(key(a[i]), i - 1, a[..], key) == position(key(a[i]), i, a[..], key) - 1) {
+ensures(position(key(a[i]), i - 1, a[..]) == position(key(a[i]), i, a[..]) - 1) {
   assert (a[..(i+1)] == a[..i] + [a[i]]);
-  numEq_app(key(a[i]), a[..i], [a[i]], key);
-  numEq_singleton(a[i], key(a[i]), key);
+  numEq_app(key(a[i]), a[..i], [a[i]]);
+  numEq_singleton(a[i], key(a[i]));
 }
 
-lemma position_decr_index_diff<T>(a : seq<T>, i : int, x : int, key: T -> int)
+lemma position_decr_index_diff(a : seq<G>, i : int, x : int)
 requires(0 <= i < |a|)
 requires(key(a[i]) != x)
-ensures(position(x, i - 1, a[..], key) == position(x, i, a[..], key)) {
+ensures(position(x, i - 1, a[..]) == position(x, i, a[..])) {
   assert (a[..(i+1)] == a[..i] + [a[i]]);
-  numEq_app(x, a[..i], [a[i]], key);
+  numEq_app(x, a[..i], [a[i]]);
   filterEmpty([a[i]], y => key(y) == x);
-  assert(numEq(x, [a[i]], key) == 0);
+  assert(numEq(x, [a[i]]) == 0);
 }
 
 predicate permutation<T>(a: seq<T>, b : seq<T>) {
@@ -371,26 +378,27 @@ ensures(forall x :: x in b ==> x in a) {
   }
 }
 
-//We define the map function and don't do too much with it (SEE)
-function mapKey<T>(a: seq<T>, key : T -> int) : seq<int> {
-    if (|a| <= 0) then [] else [key(a[0])] + mapKey(a[1..], key) 
+//In order to prove that permutations preserve the numEq, numLeq, and numLt relations, we need to relate
+//the original seq to the seq consisting of the keys. Here is a specialized map function to do that
+function mapKey(a: seq<G>) : seq<int> {
+    if (|a| <= 0) then [] else [key(a[0])] + mapKey(a[1..]) 
 }
 
-lemma mapKey_length<T>(a: seq<T>, key: T -> int) 
-ensures(|a| == |mapKey(a, key)|) {
+lemma mapKey_length(a: seq<G>) 
+ensures(|a| == |mapKey(a)|) {
 }
 
-lemma mapKey_nil<T>(a: seq<T>, key : T -> int)
+lemma mapKey_nil(a: seq<G>)
 requires(|a| == 0)
-ensures(mapKey(a, key) == []) {
+ensures(mapKey(a) == []) {
 
 }
 
-lemma mapKey_app<T>(a: seq<T>, b : seq<T>, key : T -> int)
-ensures(mapKey(a + b, key) == mapKey(a, key) + mapKey(b, key)) {
+lemma mapKey_app(a: seq<G>, b : seq<G>)
+ensures(mapKey(a + b) == mapKey(a) + mapKey(b)) {
     if(|a| <= 0) {
         assert(a == []);
-        mapKey_nil(a, key);
+        mapKey_nil(a);
         assert(a + b == b);
     }
     else {
@@ -398,44 +406,43 @@ ensures(mapKey(a + b, key) == mapKey(a, key) + mapKey(b, key)) {
     }
 }
 
-lemma mapKey_in<T>(a: seq<T>, x : T, k : int, key : T -> int)
+lemma mapKey_in(a: seq<G>, x : G, k : int)
 requires(x in a)
 requires(0 <= k < |a|)
 requires(a[k] == x)
-requires(|a| == |mapKey(a, key)|) //always true
-ensures(mapKey(a, key)[k] == key(x)) {
+requires(|a| == |mapKey(a)|) //always true but need for ensures to verify
+ensures(mapKey(a)[k] == key(x)) {
     if (|a| <= 0) {
     }
     else {
         if (k == 0) {}
         else {
-            mapKey_length(a[1..], key);
-            mapKey_in(a[1..], x, k-1, key);
-            assert(mapKey(a[1..], key)[k-1] == mapKey(a[..], key)[k]);
+            mapKey_length(a[1..]);
+            mapKey_in(a[1..], x, k-1);
+            assert(mapKey(a[1..])[k-1] == mapKey(a[..])[k]);
         }
     }
 }
 
-lemma numEq_mapKey<T>(a: seq<T>, x : int, key : T -> int)
-ensures(numEq(x, a, key) == |filter(mapKey(a, key), y => y == x)|) {
-
+lemma numEq_mapKey(a: seq<G>, x : int)
+ensures(numEq(x, a) == |filter(mapKey(a), y => y == x)|) {
 }
 
 //really annoying to prove (of couse, holds for map in general)
-lemma perm_mapKey<T>(a: seq<T>, b : seq<T>, key : T -> int) 
+lemma perm_mapKey(a: seq<G>, b : seq<G>) 
 requires(permutation(a,b))
-ensures(permutation(mapKey(a, key), mapKey(b, key))) {
+ensures(permutation(mapKey(a), mapKey(b))) {
     permutation_length(a, b);
     if (|a| <= 0) {}
     else {
         assert(a[0] in a);
-        assert(key(a[0]) in mapKey(a, key));
+        assert(key(a[0]) in mapKey(a));
         perm_in(b, a);
         assert (a[0] in b);
         assert(exists k :: 0 <= k < |b| && b[k] == a[0]);
         var k :| 0 <= k < |b| && b[k] == a[0];
-        mapKey_length(b, key);
-        mapKey_in(b, a[0], k, key);
+        mapKey_length(b);
+        mapKey_in(b, a[0], k);
         assert(b == b[..k] + [b[k]] + b[k+1..]);
         assert(a == [a[0]] + a[1..]);
         var newB := b[..k] + b[k+1..];
@@ -445,20 +452,20 @@ ensures(permutation(mapKey(a, key), mapKey(b, key))) {
         assert(multiset([b[k]]) == multiset([a[0]]));
         multiset_union_inj(multiset(a[1..]), multiset(newB), multiset([a[0]]));
         assert(multiset(a[1..]) == multiset(newB));
-        perm_mapKey(a[1..], newB, key); //use IH
-        assert(multiset(mapKey(a[1..], key)) == multiset(mapKey(newB, key)));
+        perm_mapKey(a[1..], newB); //use IH
+        assert(multiset(mapKey(a[1..])) == multiset(mapKey(newB)));
         assert(b == b[..k] + b[k..]);
-        mapKey_app(b[..k], b[k..], key);
-        multiset_app(mapKey(b[..k], key), mapKey(b[k..], key));
-        assert(multiset(mapKey(b, key)) == multiset(mapKey(b[..k], key)) + multiset(mapKey(b[k..], key)));
-        mapKey_app([a[0]], a[1..], key);
-        mapKey_app(b[..k], b[k..], key);
+        mapKey_app(b[..k], b[k..]);
+        multiset_app(mapKey(b[..k]), mapKey(b[k..]));
+        assert(multiset(mapKey(b)) == multiset(mapKey(b[..k])) + multiset(mapKey(b[k..])));
+        mapKey_app([a[0]], a[1..]);
+        mapKey_app(b[..k], b[k..]);
         assert(b[k..] == [b[k]] + b[k+1..]);
-        mapKey_app([b[k]], b[k+1..], key);
-        mapKey_app(b[..k], b[k+1..], key);
-        multiset_app(mapKey([a[0]], key), mapKey(a[1..], key));
-        multiset_app(mapKey([b[k]], key), mapKey(b[k+1..], key));
-        multiset_app(mapKey(b[..k], key), mapKey(b[k+1..], key));
+        mapKey_app([b[k]], b[k+1..]);
+        mapKey_app(b[..k], b[k+1..]);
+        multiset_app(mapKey([a[0]]), mapKey(a[1..]));
+        multiset_app(mapKey([b[k]]), mapKey(b[k+1..]));
+        multiset_app(mapKey(b[..k]), mapKey(b[k+1..]));
     }
 }
 
@@ -493,18 +500,17 @@ ensures(|filter(a, y => y == x)| == |filter(b, y => y == x)|) {
 
 }
 
-//|filter(mapKey(a, key), y => y == x)|
-
-lemma numEq_perm<T>(a:seq<T>, b : seq<T>, x : int, key : T -> int)
+//why we needed the perm_mapKey lemma
+lemma numEq_perm(a:seq<G>, b : seq<G>, x : int)
 requires(permutation(a,b))
-ensures(numEq(x, a, key) == numEq(x, b, key)) {
-    perm_mapKey(a, b, key);
-    numEq_mapKey(a, x, key);
-    numEq_mapKey(b, x, key);
-    perm_preserves_filter_eq(mapKey(a, key), mapKey(b, key), x);
+ensures(numEq(x, a) == numEq(x, b)) {
+    perm_mapKey(a, b);
+    numEq_mapKey(a, x);
+    numEq_mapKey(b, x);
+    perm_preserves_filter_eq(mapKey(a), mapKey(b), x);
 }
 
-lemma perm_preserve_pred<T>(a:seq<T>, b:seq<T>, f: T -> bool)
+lemma perm_preserve_pred(a:seq<G>, b:seq<G>, f: G -> bool)
 requires(permutation(a, b))
 requires(forall x :: x in a ==> f(x))
 ensures(forall x :: x in b ==> f(x)) {
@@ -513,36 +519,36 @@ ensures(forall x :: x in b ==> f(x)) {
   }
 }
 
-//This is really true without the lower bound but it is much easier to prove this way, and it is OK because all elts are positive anyway
-lemma {:induction x} numLt_perm<T>(a: seq<T>, b: seq<T>, x : int, key : T -> int)
+//This is really true without the nonnegative requirement (we can't induct on x otherwise) but it is much easier to prove this way, and it is OK because all elts are positive anyway
+lemma {:induction x} numLt_perm(a: seq<G>, b: seq<G>, x : int)
 requires (permutation(a, b))
 requires(forall x :: x in a ==> key(x) >= 0)
-ensures(numLt(x, a, key) == numLt(x, b, key)) {
+ensures(numLt(x, a) == numLt(x, b)) {
   if(x <= 0) {
     filterEmpty(a, y => key(y) < x);
     perm_preserve_pred(a, b, y => key(y) >= 0);
     filterEmpty(b, y => key(y) < x);
   }
   else {
-    numLt_ind(x, a, key);
-    numLt_ind(x, b, key);
-    numLt_perm(a, b, x-1, key);
-    assert(numLt(x, a, key) == |filter(a, y => key(y) < x)|);
-    assert(numLt(x, b, key) == |filter(b, y => key(y) < x)|);
-    numEq_perm(a, b, x-1, key);
-    assert(numEq(x-1, a, key) == numEq(x-1, b, key));
+    numLt_ind(x, a);
+    numLt_ind(x, b);
+    numLt_perm(a, b, x-1);
+    assert(numLt(x, a) == |filter(a, y => key(y) < x)|);
+    assert(numLt(x, b) == |filter(b, y => key(y) < x)|);
+    numEq_perm(a, b, x-1);
+    assert(numEq(x-1, a) == numEq(x-1, b));
     perm_in(a, b);
     perm_in(b,a);
   }
 }
 
 //numLeq is also preserved over permutations
-lemma numLeq_perm<T>(a: seq<T>, b: seq<T>, x : int, key : T -> int)
+lemma numLeq_perm(a: seq<G>, b: seq<G>, x : int)
 requires (permutation(a, b))
-requires(forall x : T :: x in a ==> key(x) >= 0)
-ensures(numLeq(x, a, key) == numLeq(x, b, key)) {
-  numLt_perm(a, b, x, key);
-  numEq_perm(a, b, x, key);
+requires(forall x :: x in a ==> key(x) >= 0)
+ensures(numLeq(x, a) == numLeq(x, b)) {
+  numLt_perm(a, b, x);
+  numEq_perm(a, b, x);
   perm_in(a,b);
   perm_in(b,a);
 }
@@ -563,58 +569,58 @@ ensures(forall i :: 0 <= i < a.Length ==> f(a[i])) {
 
 // Sortedness - two equivalent definitions 
 
-//A sequence is sorted if the expected condition is satisfied - ie, if i <= j, a[i] <= a[j]
-predicate sorted<T>(a: seq<T>, key : T -> int) {
+//we sort sequences by keys
+predicate sorted(a: seq<G>) {
   forall i : int, j : int :: 0 <= i < |a| ==> 0 <= j < |a| && i <= j ==> key(a[i]) <= key(a[j])
 }
 
 //alternate sorting condition - if every element is at one of its possible correct positions in the array, then the array is sorted
 //  generalization of version in DistinctElts, because an element can be in a range of possible positions
-predicate sorted_alt<T>(a:seq<T>, key : T -> int) {
-  forall i : int :: 0 <= i < |a| ==> numLt(key(a[i]), a[..], key) <= i <= numLeq(key(a[i]), a[..], key) - 1
+predicate sorted_alt(a:seq<G>) {
+  forall i : int :: 0 <= i < |a| ==> numLt(key(a[i]), a[..]) <= i <= numLeq(key(a[i]), a[..]) - 1
 }
 
 //The only direction we need - if a sequence satsifies [sorted_alt(a)], then it satisfies [sorted(a)]
-lemma sorted_alt_implies_sorted<T>(a: seq<T>, key : T -> int)
-requires(sorted_alt(a, key))
-ensures(sorted(a, key)) {
+lemma sorted_alt_implies_sorted(a: seq<G>)
+requires(sorted_alt(a))
+ensures(sorted(a)) {
   forall i : int, j : int | 0 <= i < |a| && 0 <= j < |a| && i <= j
     ensures(key(a[i]) <= key(a[j])) {
       if(key(a[j]) < key(a[i])) {
-        numLt_leq_bound(a, key(a[j]), key(a[i]), key);
+        numLt_leq_bound(a, key(a[j]), key(a[i]));
       }
       else {
       }
     }
 }
 
-//We use a stronger invariant, so we want to show that this implies sorting
-lemma all_positions_implies_sorted<T>(a : seq<T>, c : seq<T>, key : T -> int)
+//We use a stronger invariant, so we want to show that this implies sorting_alt (and thus sorted)
+lemma all_positions_implies_sorted(a : seq<G>, c : seq<G>)
 requires(permutation(a, c))
 requires(|a| == |c|)
 requires(forall x :: x in a ==> key(x) >= 0)
-requires(forall j :: 0 <= j < |c| ==> exists k :: ((-1 < k < |a|) && c[j] == a[k] && j == position(key(a[k]), k, a[..], key)))
-ensures(sorted_alt(c, key)) {
+requires(forall j :: 0 <= j < |c| ==> exists k :: ((-1 < k < |a|) && c[j] == a[k] && j == position(key(a[k]), k, a[..])))
+ensures(sorted_alt(c)) {
   forall i : int | 0 <= i < |a|
-  ensures(numLt(key(c[i]), c[..], key) <= i <= numLeq(key(c[i]), c[..], key) - 1) {
+  ensures(numLt(key(c[i]), c[..]) <= i <= numLeq(key(c[i]), c[..]) - 1) {
     assert(0 <= i < |c|);
-    var k :| (-1 < k < |a|) && c[i] == a[k] && i == position(key(a[k]), k, a[..], key);
-    position_bounds(a, a[k], k, key);
-    numLt_perm(a, c, key(c[i]), key);
-    numEq_perm(a, c, key(c[i]), key);
+    var k :| (-1 < k < |a|) && c[i] == a[k] && i == position(key(a[k]), k, a[..]);
+    position_bounds(a, a[k], k);
+    numLt_perm(a, c, key(c[i]));
+    numEq_perm(a, c, key(c[i]));
   }
 }
 
 //If the [sorted_alt] condition holds on an array, then it holds on the seq version of the array too
-lemma sorted_alt_seq_array<T>(a: array<T>, key : T -> int) 
-requires(forall i : int :: 0 <= i < a.Length ==> numLt(key(a[i]), a[..], key) <= i <= numLeq(key(a[i]), a[..], key) - 1)
-ensures(sorted_alt(a[..], key)){
+lemma sorted_alt_seq_array(a: array<G>) 
+requires(forall i : int :: 0 <= i < a.Length ==> numLt(key(a[i]), a[..]) <= i <= numLeq(key(a[i]), a[..]) - 1)
+ensures(sorted_alt(a[..])){
 }
 
 // Stability = we say that a and b are stable with respect to each other if the relative order of equal elements is preseved
 //  We can express that as the following 
 
-predicate stable<T>(a : seq<T>, b : seq<T>, key : T -> int) {
+predicate stable(a : seq<G>, b : seq<G>) {
   forall x : int :: filter(a, y => key(y) == x) == filter(b, y => key(y) == x)
 }
 /* Lemmas to prove function invariants */
@@ -626,9 +632,9 @@ ensures(filter(a[..i+1], f) == filter(a[..i], f) + filter([a[i]], f)) {
   filter_app(a[..i], [a[i]], f);
 }
 
-lemma numEq_split_idx<T>(a: array<T>, i : int, key : T -> int) 
+lemma numEq_split_idx(a: array<G>, i : int) 
 requires(0 <= i < a.Length)
-ensures(forall j :: numEq(j, a[..i+1], key) == numEq(j, a[..i], key) + numEq(j, [a[i]], key)) {
+ensures(forall j :: numEq(j, a[..i+1]) == numEq(j, a[..i]) + numEq(j, [a[i]])) {
   forall j  {
     filter_split_idx(a, y => key(y) == j, i);
   }
@@ -637,20 +643,20 @@ ensures(forall j :: numEq(j, a[..i+1], key) == numEq(j, a[..i], key) + numEq(j, 
 //The first loop of countingSort - builds an array that counts the occurrences of each element 
 
 //Prove the invariant is preserved through the loop in a separate lemma, since Dafny has trouble proving it automatically
-lemma countOccurrencesInvariant<T>(a : array<T>, b : seq<int>, newB : seq<int>, i : int, elt: int, key : T -> int)
+lemma countOccurrencesInvariant(a : array<G>, b : seq<int>, newB : seq<int>, i : int, elt: int)
 requires(0 <= i < a.Length)
 requires(0 <= key(a[i]) < |b|)
 requires(|b| == |newB|)
 requires(key(a[i]) == elt)
 requires(newB == b[elt := b[elt]   + 1])
-requires(forall j :: 0 <= j < |b| ==> b[j] == numEq(j, a[..i], key))
-ensures(forall j :: 0 <= j < |newB| ==> newB[j] == numEq(j, a[..i+1], key)) {
+requires(forall j :: 0 <= j < |b| ==> b[j] == numEq(j, a[..i]))
+ensures(forall j :: 0 <= j < |newB| ==> newB[j] == numEq(j, a[..i+1])) {
   forall j | 0 <= j <|newB|
-  ensures(newB[j] == numEq(j, a[..i+1], key)) {
+  ensures(newB[j] == numEq(j, a[..i+1])) {
     assert(a[..i+1] == a[..i] + [a[i]]);
-    numEq_app(j, a[..i], [a[i]], key);
+    numEq_app(j, a[..i], [a[i]]);
     if(j == elt) {
-      numEq_singleton(a[i], key(a[i]), key);
+      numEq_singleton(a[i], key(a[i]));
       assert(newB[j] == b[elt] + 1);  
     }
     else {
@@ -659,54 +665,54 @@ ensures(forall j :: 0 <= j < |newB| ==> newB[j] == numEq(j, a[..i+1], key)) {
   }
 }
 
-method countOccurrences<T> (a: array<T>, k: int, key : T -> int) returns (b: array<int>)
+method countOccurrences(a: array<G>, k: int) returns (b: array<int>)
 requires 0 < a.Length
 requires 0 < k
 requires (forall i: int :: 0 <= i < a.Length ==> 0 <= key(a[i]) < k)
 ensures (b.Length == k + 1)
-ensures(forall i : int :: 0 <= i <= k ==> b[i] == numEq(i, a[..], key))
+ensures(forall i : int :: 0 <= i <= k ==> b[i] == numEq(i, a[..]))
 {
   b := new int[k+1](i => 0);
   var i := 0;
   while(i < a.Length) 
   decreases(a.Length - i)
   invariant (0 <= i <= a.Length)
-  invariant(forall j : int :: 0 <= j <= k ==> b[j] == numEq(j, a[..i], key)) {
+  invariant(forall j : int :: 0 <= j <= k ==> b[j] == numEq(j, a[..i])) {
     ghost var oldB := b[..];
     ghost var ai := key(a[i]);
     b[key(a[i])] := b[key(a[i])] + 1;
 
     assert(b[..] == oldB[ai := oldB[ai] + 1]);
-    countOccurrencesInvariant(a, oldB, b[..], i, key(a[i]), key);
+    countOccurrencesInvariant(a, oldB, b[..], i, key(a[i]));
 
     i := i + 1;
-    assert(forall j : int :: 0 <= j <= k ==> b[j] == numEq(j, a[..i], key)); //for some reason, need this for it to verify
+    assert(forall j : int :: 0 <= j <= k ==> b[j] == numEq(j, a[..i])); //for some reason, need this for it to verify
   }
   assert(a[..i] == a[..]);
 }
 
 
 //The second loop in countingSort - returns array which gives positions of elements in sorted array//
-method prefixSum<T>(a:array<T>, b : array<int>, key : T -> int) returns (c: array<int>)
+method prefixSum(a:array<G>, b : array<int>) returns (c: array<int>)
 requires(0 < b.Length)
-requires(forall i : int :: 0 <= i < b.Length ==> b[i] == numEq(i, a[..], key))
+requires(forall i : int :: 0 <= i < b.Length ==> b[i] == numEq(i, a[..]))
 requires (forall i: int :: 0 <= i < a.Length ==> 0 <= key(a[i]))
 ensures(c.Length == b.Length)
-ensures(forall i : int {:induction i} :: 0 <= i < b.Length ==> (c[i] == numLeq(i, a[..], key) - 1));
+ensures(forall i : int {:induction i} :: 0 <= i < b.Length ==> (c[i] == numLeq(i, a[..]) - 1));
 {
   var i := 1;
   //need to know that there are no elements less than x
-  numLt_unfold_zero(a[..], key);
+  numLt_unfold_zero(a[..]);
   filterEmpty(a[..], y => key(y) < 0);
-  assert(numLeq(0, a[..], key) == b[0]);
+  assert(numLeq(0, a[..]) == b[0]);
   c := new int[b.Length];
   c[0] := b[0] - 1;
   while(i < c.Length)
   decreases (b.Length - i)
   invariant (1 <= i <= c.Length)
-  invariant(forall j: int {:induction j} :: (0 <= j < i ==> c[j] == numLeq(j, a[..], key) - 1))
+  invariant(forall j: int {:induction j} :: (0 <= j < i ==> c[j] == numLeq(j, a[..]) - 1))
   {
-    numLeq_ind(i, a[..], key);
+    numLeq_ind(i, a[..]);
     c[i] := b[i] + c[i-1];
     i := i + 1;
   }
@@ -718,12 +724,12 @@ ensures(forall i : int {:induction i} :: 0 <= i < b.Length ==> (c[i] == numLeq(i
 //  of the nontrivial work (invariant preservation, proving postconditions, proving key properties) in the following lemmas.
 
 //The array b is correct to begin
-lemma constructSortedArrayBInvarEntry<T>(a: array<T>, b : array<int>, i : int, key : T -> int)
-requires (forall j :: 0 <= j < b.Length ==> b[j] == numLeq(j, a[..], key) - 1)
+lemma constructSortedArrayBInvarEntry(a: array<G>, b : array<int>, i : int)
+requires (forall j :: 0 <= j < b.Length ==> b[j] == numLeq(j, a[..]) - 1)
 requires(i == a.Length - 1)
-ensures (forall j :: 0 <= j < b.Length ==> b[j] == numLt(j, a[..], key) + numEq(j, a[..(i+1)], key) - 1) {
+ensures (forall j :: 0 <= j < b.Length ==> b[j] == numLt(j, a[..]) + numEq(j, a[..(i+1)]) - 1) {
     forall j | 0 <= j < b.Length
-    ensures (b[j] == numLt(j, a[..], key) + numEq(j, a[..(i+1)], key) - 1) {
+    ensures (b[j] == numLt(j, a[..]) + numEq(j, a[..(i+1)]) - 1) {
         assert (a[..(i+1)] == a[..]);
     }
 }
@@ -732,23 +738,23 @@ ensures (forall j :: 0 <= j < b.Length ==> b[j] == numLt(j, a[..], key) + numEq(
 
 
 //A key lemma: in our loop, c[b1[a]] != -1, so we do not overwrite a previously written value
-//NOTE: for default - plan is to require a default where key(default) == -1
-lemma sortedArrayLoopSeesNewElt<T>(a: array<T>, b: array<int>, c: array<T>, i : int, default : T, key : T -> int)
+//NOTE: for default - plan is to require a default where key(default) < 0
+lemma sortedArrayLoopSeesNewElt(a: array<G>, b: array<int>, c: array<G>, i : int, default : G)
 requires(a.Length == c.Length)
 requires(0 <= i < a.Length)
-requires(forall x : T :: x in a[..] ==> x != default)
-requires(forall j :: 0 <= j < c.Length ==> c[j] != default ==> exists k :: ((i < k < a.Length) && c[j] == a[k] && j == position(key(a[k]), k, a[..], key)))
-requires((forall j :: 0 <= j < b.Length ==> b[j] == position(j, i, a[..], key)))
+requires(forall x :: x in a[..] ==> x != default)
+requires(forall j :: 0 <= j < c.Length ==> c[j] != default ==> exists k :: ((i < k < a.Length) && c[j] == a[k] && j == position(key(a[k]), k, a[..])))
+requires((forall j :: 0 <= j < b.Length ==> b[j] == position(j, i, a[..])))
 requires(0 <= key(a[i]) < b.Length)
 requires(0 <= b[key(a[i])] < c.Length)
 ensures(c[b[key(a[i])]] == default) {
   //pf by contradiction
   if(c[b[key(a[i])]] == default) {}
   else {
-    var k :| (i < k < a.Length) && c[b[key(a[i])]] == a[k] && b[key(a[i])] == position(key(a[k]), k, a[..], key);
-    assert(b[key(a[i])] == position(key(a[k]), k, a[..], key));
-    assert(b[key(a[i])] == position(key(a[i]), i, a[..], key));
-    position_inj(a[..], i, k, key);
+    var k :| (i < k < a.Length) && c[b[key(a[i])]] == a[k] && b[key(a[i])] == position(key(a[k]), k, a[..]);
+    assert(b[key(a[i])] == position(key(a[k]), k, a[..]));
+    assert(b[key(a[i])] == position(key(a[i]), i, a[..]));
+    position_inj(a[..], i, k);
   }
 }
 
@@ -758,7 +764,7 @@ requires (0 <= i < |a|)
 ensures(a == a[..i] + [a[i]] + a[i+1..]) {}
 
 //The permutation invariant: the completed part of c is a permutation of a[(i+1)..]
-lemma permutation_invariant<T>(a: array<T>, c : seq<T>, oldC : seq<T>, idx : int, i : int, default : T, key : T -> int)
+lemma permutation_invariant(a: array<G>, c : seq<G>, oldC : seq<G>, idx : int, i : int, default : G)
 requires(0 <= i < a.Length)
 requires(a.Length == |c|)
 requires(|c| == |oldC|)
@@ -793,7 +799,7 @@ ensures(permutation(a[i..], filter(c, y => y != default))) {
 }
 
 //The invariant that the length of the completed part of c is |a| - (i+1)
-lemma filter_length_invariant<T>(a: array<T>, c : seq<T>, oldC : seq<T>, idx : int, i : int, default : T, key : T -> int)
+lemma filter_length_invariant(a: array<G>, c : seq<G>, oldC : seq<G>, idx : int, i : int, default : G)
 requires(0 <= i < a.Length)
 requires(a.Length == |c|)
 requires(|c| == |oldC|)
@@ -821,53 +827,53 @@ ensures(|filter(c[..], y => y != default)| == a.Length - i) {
 
 
 //The values in the b array are bounded (used for array bounds)
-lemma b_bound_invariant<T>(a: array<T>, oldB : seq<int>, b : seq<int>, i: int, idx : int, key : T -> int)
+lemma b_bound_invariant(a: array<G>, oldB : seq<int>, b : seq<int>, i: int, idx : int)
 requires(0 <= i < a.Length)
 requires(0 <= key(a[i]) < |oldB|)
 requires(|b| == |oldB|)
 requires(b[key(a[i])] == idx - 1)
 requires(forall j :: 0 <= j < |b| ==> j != key(a[i]) ==> b[j] == oldB[j]);
 requires(idx == oldB[key(a[i])])
-requires(forall j : int :: 0 <= j < |oldB| ==> oldB[j] <= numLeq(j, a[..], key) - 1)
-ensures((forall j : int :: 0 <= j < |b| ==> b[j] <= numLeq(j, a[..], key) - 1)){
+requires(forall j : int :: 0 <= j < |oldB| ==> oldB[j] <= numLeq(j, a[..]) - 1)
+ensures((forall j : int :: 0 <= j < |b| ==> b[j] <= numLeq(j, a[..]) - 1)){
 }
 
 //Invariant that the array "b" consists of the positions of all elements, only considering equal elements up to index i
-lemma b_position_invariant<T>(a:array<T>, oldB : seq<int>, b : seq<int>, i : int, idx : int, key : T -> int)
+lemma b_position_invariant(a:array<G>, oldB : seq<int>, b : seq<int>, i : int, idx : int)
 requires(0 <= i < a.Length)
 requires(0 <= key(a[i]) < |oldB|)
 requires(|b| == |oldB|)
 requires(b[key(a[i])] == idx - 1)
 requires(forall j :: 0 <= j < |b| ==> j != key(a[i]) ==> b[j] == oldB[j]);
 requires(idx == oldB[key(a[i])])
-requires(forall j :: 0 <= j < |oldB| ==> oldB[j] == position(j, i, a[..], key));
-ensures(forall j :: 0 <= j < |b| ==> b[j] == position(j, i-1, a[..], key)) {
+requires(forall j :: 0 <= j < |oldB| ==> oldB[j] == position(j, i, a[..]));
+ensures(forall j :: 0 <= j < |b| ==> b[j] == position(j, i-1, a[..])) {
   forall j | 0 <= j < |b| 
-  ensures(b[j] == position(j, i-1, a[..], key)) {
+  ensures(b[j] == position(j, i-1, a[..])) {
     if(j == key(a[i])) {
       assert(b[j] == oldB[j] - 1);
-      position_decr_index_same(a[..], i, key);
-      assert(position(j, i-1, a[..], key) == position(j, i, a[..], key) - 1);
+      position_decr_index_same(a[..], i);
+      assert(position(j, i-1, a[..]) == position(j, i, a[..]) - 1);
     }
     else {
-      position_decr_index_diff(a[..], i, j, key);
+      position_decr_index_diff(a[..], i, j);
     }
   }
 }
 
 //The important invariant for sorting and stability: each element c[j] corresponds to the element of k actually at position j in a sorted array
-lemma c_structure_invariant<T>(a: array<T>, b: seq<int>, c : seq<T>, oldC: seq<T>, idx : int, i : int, default : T, key : T -> int)
+lemma c_structure_invariant(a: array<G>, b: seq<int>, c : seq<G>, oldC: seq<G>, idx : int, i : int, default : G)
 requires(0 <= i < a.Length)
 requires(0 <= key(a[i]) < |b|)
 requires(a.Length == |c|)
 requires(idx == b[key(a[i])])
-requires(idx == position(key(a[i]), i, a[..], key))
+requires(idx == position(key(a[i]), i, a[..]))
 requires(|c| == |oldC|)
 requires(0 <= idx < a.Length)
 requires(c == oldC[idx := a[i]])
 requires(forall x :: x in a[..] ==> x != default)
-requires(forall j :: 0 <= j < |oldC| ==> oldC[j] != default ==> exists k :: ((i < k < a.Length) && oldC[j] == a[k] && j == position(key(a[k]), k, a[..], key)))
-ensures(forall j :: 0 <= j < |c| ==> c[j] != default ==> exists k :: ((i-1 < k < a.Length) && c[j] == a[k] && j == position(key(a[k]), k, a[..], key))) {
+requires(forall j :: 0 <= j < |oldC| ==> oldC[j] != default ==> exists k :: ((i < k < a.Length) && oldC[j] == a[k] && j == position(key(a[k]), k, a[..])))
+ensures(forall j :: 0 <= j < |c| ==> c[j] != default ==> exists k :: ((i-1 < k < a.Length) && c[j] == a[k] && j == position(key(a[k]), k, a[..]))) {
   forall j | 0 <= j < |c| && c[j] != default
   ensures(exists k :: (i-1 < k < a.Length) && c[j] == a[k]) {
     if(j != idx) {
@@ -875,7 +881,7 @@ ensures(forall j :: 0 <= j < |c| ==> c[j] != default ==> exists k :: ((i-1 < k <
     else {
       assert(-1 < i < a.Length);
       assert(c[j] == a[i]);
-      assert(j == position(key(a[i]), i, a[..], key));
+      assert(j == position(key(a[i]), i, a[..]));
     }
   }
 }
@@ -883,7 +889,7 @@ ensures(forall j :: 0 <= j < |c| ==> c[j] != default ==> exists k :: ((i-1 < k <
 //Prove that the invariants imply the postconditions in a separate lemma
 
 //Our loop invariants imply the output is a permutation of the input
-lemma afterLoopPermutation<T>(a: array<T>, c : array<T>, default : T, key : T -> int)
+lemma afterLoopPermutation(a: array<G>, c : array<G>, default : G)
 requires(permutation((a[0..]),(filter(c[..], y => y != default)))) //permutation invariant
 requires(a.Length == c.Length)
 ensures(permutation(a[..], c[..])) {
@@ -893,30 +899,29 @@ ensures(permutation(a[..], c[..])) {
 }
 
 //Our loops invariants imply the output is sorted
-lemma afterLoopSorted<T>(a : array<T>, c : array<T>, default : T, key : T -> int)
+lemma afterLoopSorted(a : array<G>, c : array<G>, default : G)
 requires(forall x :: x in a[..] ==> key(x) >= 0)
 requires(|filter(c[..], y => y != default)| == a.Length)
 requires(permutation(a[..], c[..]))
 requires(a.Length == c.Length)
-requires(forall j :: 0 <= j < c.Length ==> c[j] != default ==> exists k :: ((-1 < k < a.Length) && c[j] == a[k] && j == position(key(a[k]), k, a[..], key)))
-ensures(sorted(c[..], key)) {
+requires(forall j :: 0 <= j < c.Length ==> c[j] != default ==> exists k :: ((-1 < k < a.Length) && c[j] == a[k] && j == position(key(a[k]), k, a[..])))
+ensures(sorted(c[..])) {
   filter_same_length_all(c[..], y => y != default); //the filtered list is the original list
   filterAll(c[..], y => y != default);
   all_elems_seq_array(c, y => y != default); //all elements in c satsify y >= 0
-  all_elems_seq_array(c, y => y != default);
+  //all_elems_seq_array(c, y => y != default);
   assert(forall j :: 0 <= j  < c.Length ==> c[j] != default);
-  assert(forall j :: 0 <= j < c.Length ==> exists k :: ((-1 < k < a.Length) && c[j] == a[k] && j == position(key(a[k]), k, a[..], key)));
-  all_positions_implies_sorted(a[..], c[..], key);
-  assert(sorted_alt(c[..], key)); 
-  sorted_alt_seq_array(c, key); //c[..] satsifes sorted_alt condition
-  sorted_alt_implies_sorted(c[..], key); //c[..] is sorted
+  assert(forall j :: 0 <= j < c.Length ==> exists k :: ((-1 < k < a.Length) && c[j] == a[k] && j == position(key(a[k]), k, a[..])));
+  all_positions_implies_sorted(a[..], c[..]);
+  assert(sorted_alt(c[..])); 
+  sorted_alt_seq_array(c); //c[..] satsifes sorted_alt condition
+  sorted_alt_implies_sorted(c[..]); //c[..] is sorted
 }
 
-lemma no_default_elts<T>(a: array<T>, default : T, key : T -> int)
+lemma no_default_elts(a: array<G>, default : G)
 requires(forall j :: 0 <= j < a.Length ==> 0 <= key(a[j])); 
 requires(key(default) < 0)
-ensures(forall x : T :: x in a[..] ==> x != default) {
-
+ensures(forall x :: x in a[..] ==> x != default) {
 }
 
 // Proofs for stability 
@@ -926,7 +931,7 @@ ensures(forall x : T :: x in a[..] ==> x != default) {
 
 //first, we need to know that at any point in the loop, for all j < b[a[i]], c[j] != a[i] - ie, the current element is the
 //first one in the current array with that value - because we go backwards, this ensures stability
-lemma all_same_elts_come_after<T>(a: array<T>, oldC : seq<T>, i : int, ai : T, bai : int, default : T, key : T -> int)
+lemma all_same_elts_come_after(a: array<G>, oldC : seq<G>, i : int, ai : G, bai : int, default : G)
 requires(0 <= i < a.Length)
 requires(ai == a[i])
 requires(0 <= key(ai))
@@ -934,22 +939,23 @@ requires(0 <= key(ai))
 requires(key(default) < 0)
 // /requires(0 <= ai < |b|)
 //requires(bai == b[ai])
-requires(bai == position(key(ai), i, a[..], key))
+requires(bai == position(key(ai), i, a[..]))
 requires(0 <= bai < |oldC|)
 requires(a.Length == |oldC|)
-requires(forall j :: 0 <= j < |oldC| ==> oldC[j] != default ==> exists k :: ((i < k < a.Length) && oldC[j] == a[k] && j == position(key(a[k]), k, a[..], key)))
+requires(forall j :: 0 <= j < |oldC| ==> oldC[j] != default ==> exists k :: ((i < k < a.Length) && oldC[j] == a[k] && j == position(key(a[k]), k, a[..])))
 ensures(forall j :: 0 <= j < bai ==> key(oldC[j]) != key(a[i])) {
   forall j | 0 <= j < bai
   ensures(key(oldC[j]) != key(a[i])) {
     if(key(oldC[j]) == key(a[i])) {
       //assert(oldC[j] != default);
-      var k :| ((i < k < a.Length) && oldC[j] == a[k] && j == position(key(a[k]), k, a[..], key));
-      assert(position(key(a[i]), k, a[..], key) < position(key(a[i]), i, a[..], key));
-      positions_eq_preserve_order((a[..]), k, i, a[i], key);
+      var k :| ((i < k < a.Length) && oldC[j] == a[k] && j == position(key(a[k]), k, a[..]));
+      assert(position(key(a[i]), k, a[..]) < position(key(a[i]), i, a[..]));
+      positions_eq_preserve_order((a[..]), k, i, a[i]);
     }
     else {}
   }
 }
+
 /*
 lemma no_elts_come_before<T>(a: array<T>, oldC : seq<T>, i : int, ai : T, bai : int, default : T, key : T -> int)
 requires(0 <= i < a.Length)
@@ -966,16 +972,16 @@ ensures(forall j :: 0 <= j < bai ==> oldC[j] != a[i]) {
 
 }*/
 
-lemma filter_filter_special<T>(a: seq<T>, default : T, x: int, key : T -> int)
+lemma filter_filter_special(a: seq<G>, default : G, x: int)
 ensures(filter((filter(a, y => y != default)), y => key(y) == x) == filter(a, y => y != default && key(y) == x)) {
 }
 
-lemma stable_invariant_preserved<T>(a: array<T>, b : seq<int>, oldC : seq<T>, c : seq<T>, i : int, ai: T, bai : int, default: T, key : T -> int)
+lemma stable_invariant_preserved(a: array<G>, b : seq<int>, oldC : seq<G>, c : seq<G>, i : int, ai: G, bai : int, default: G)
 requires(0 <= i < a.Length)
 requires(ai == a[i])
 requires(0 <= key(ai) < |b|)
 requires(bai == b[key(a[i])])
-requires(bai == position(key(ai), i, a[..], key))
+requires(bai == position(key(ai), i, a[..]))
 requires(0 <= bai < |c|)
 requires(a.Length == |c|)
 requires(|c| == |oldC|)
@@ -983,14 +989,14 @@ requires(oldC[bai] == default)
 requires(c == oldC[bai := ai])
 requires(a[i] != default)
 requires(key(default) < 0)
-requires(forall j :: 0 <= j < |oldC| ==> oldC[j] != default ==> exists k :: ((i < k < a.Length) && oldC[j] == a[k] && j == position(key(a[k]), k, a[..], key)))
+requires(forall j :: 0 <= j < |oldC| ==> oldC[j] != default ==> exists k :: ((i < k < a.Length) && oldC[j] == a[k] && j == position(key(a[k]), k, a[..])))
 requires(forall x : int :: filter(a[i+1..], y => key(y) == x) == filter(filter(oldC, y => y != default), y => key(y) == x))
 ensures(forall x : int :: filter(a[i..], y => key(y) == x) == filter(filter(c, y => y != default), y => key(y) == x)) {
   forall x 
   ensures (filter(a[i..], y => key(y) == x) == filter(filter(c, y => y != default), y => key(y) == x)) {
     assert(filter(a[i+1..], y => key(y) == x) == filter(filter(oldC, y => y != default), y => key(y) == x));
-    filter_filter_special(c, default, x, key);
-    filter_filter_special(oldC, default, x, key);
+    filter_filter_special(c, default, x);
+    filter_filter_special(oldC, default, x);
     assert(a[i..] == [a[i]] + a[i+1..]);
     filter_app([a[i]], a[i+1..], y => key(y) == x);
     filter_app(c[..b[key(a[i])]], c[b[key(a[i])]..], y => (y != default && key(y) == x));
@@ -1011,7 +1017,7 @@ ensures(forall x : int :: filter(a[i..], y => key(y) == x) == filter(filter(c, y
     
     if(x == key(a[i])) {
       //idea: filter(c[..b[a[i]]]) = [] and same for oldC by [all_same_elts_come_after] - the rest is easy
-      all_same_elts_come_after(a, oldC, i, a[i], b[key(a[i])], default, key);
+      all_same_elts_come_after(a, oldC, i, a[i], b[key(a[i])], default);
       assert(forall j :: 0 <= j < b[key(a[i])] ==> key(c[j]) != x);
       
       filterEmpty(c[..b[key(a[i])]], y => (y != default && key(y) == x));
@@ -1039,27 +1045,26 @@ ensures(forall x : int :: filter(a[i..], y => key(y) == x) == filter(filter(c, y
 }
 
 
-lemma afterLoopStable<T>(a : array<T>, c : array<T>, default : T, key : T -> int)
+lemma afterLoopStable(a : array<G>, c : array<G>, default : G)
 requires(a.Length == c.Length)
 requires(forall x : int :: filter(a[..], y => key(y) == x) == filter(filter(c[..], y => y != default), y => key(y) == x))
 requires(|filter(c[..], y => y != default)| == a.Length)
-ensures(stable(a[..], c[..], key)) {
+ensures(stable(a[..], c[..])) {
     filter_same_length_all(c[..], y => y != default);
     filterAll(c[..], y => y != default);
     assert((filter(c[..], y => y != default) == c[..]));
 }
 
-
 //The third (and much more complicated) loop of counting sort: put each element in its correct position 
 //a is the original array, b is prefix sum array 
 
-method constructSortedArray<T>(a: array<T>, b: array<int>, default : T, key : T -> int) returns (c : array<T>)
-requires(forall i : int {:induction i} :: 0 <= i < b.Length ==> (b[i] == numLeq(i, a[..], key) - 1));
+method constructSortedArray(a: array<G>, b: array<int>, default : G) returns (c : array<G>)
+requires(forall i : int {:induction i} :: 0 <= i < b.Length ==> (b[i] == numLeq(i, a[..]) - 1));
 requires(forall i : int :: 0 <= i < a.Length ==> 0 <= key(a[i]) < b.Length)
 requires(key(default) < 0)
-//ensures(permutation(a[..], c[..]))
-//ensures(sorted(c[..], key))
-//ensures(stable(a[..], c[..], key))
+ensures(permutation(a[..], c[..]))
+ensures(sorted(c[..]))
+ensures(stable(a[..], c[..]))
 {
   //we copy b into a new array becaues Dafny really doesnt like it when you modify inputs in the function; it has
   //difficulty proving lots of things
@@ -1072,10 +1077,10 @@ requires(key(default) < 0)
     i := i + 1;
   }
   assert(forall i :: 0 <= i < b1.Length ==> b1[i] == b[i]);
-  assert(forall i :: 0 <= i < b1.Length ==> b1[i] == numLeq(i, a[..], key) - 1);
+  assert(forall i :: 0 <= i < b1.Length ==> b1[i] == numLeq(i, a[..]) - 1);
   assert(forall i : int :: 0 <= i < a.Length ==> 0 <= key(a[i]) < b1.Length);
 
-  c := new T[a.Length](i => default);
+  c := new G[a.Length](i => default);
   i := a.Length - 1;
   //establish loop invariants
   assert(a[(i+1)..a.Length] == []);
@@ -1083,7 +1088,7 @@ requires(key(default) < 0)
   filterEmpty(c[..], y => y != default);
   
   //establish the b invariant
-  constructSortedArrayBInvarEntry(a, b1, i, key);
+  constructSortedArrayBInvarEntry(a, b1, i);
   
   //ghost var bLen := b.Length;
 
@@ -1095,37 +1100,26 @@ requires(key(default) < 0)
   invariant(-1 <= i < a.Length)
   invariant(b1.Length == b.Length) //need for bounds
   invariant(forall j :: 0 <= j < a.Length ==> 0 <= key(a[j]) < b1.Length); //also need for bounds
-  invariant(forall j : int :: 0 <= j < b1.Length ==> b1[j] <= numLeq(j, a[..], key) - 1) //used for bounds checks
+  invariant(forall j : int :: 0 <= j < b1.Length ==> b1[j] <= numLeq(j, a[..]) - 1) //used for bounds checks
   //technically, this invariant is implied by the next one (by permutation_length), but the proofs are much faster if we include both
   invariant(|filter(c[..], y => y != default)| == a.Length - (i + 1)); //ensures that we fill all of c
   invariant(permutation((a[(i+1)..]),(filter(c[..], y => y != default)))) //permutation invariant
-  invariant(forall j :: 0 <= j < b.Length ==> b1[j] == position(j, i, a[..], key)) //the array b at each step (b is changing)
-  invariant(forall j :: 0 <= j < c.Length ==> c[j] != default ==> exists k :: ((i < k < a.Length) && c[j] == a[k] && j == position(key(a[k]), k, a[..], key))) //every filled in element of c is a previously seen elt
+  invariant(forall j :: 0 <= j < b.Length ==> b1[j] == position(j, i, a[..])) //the array b at each step (b is changing)
+  invariant(forall j :: 0 <= j < c.Length ==> c[j] != default ==> exists k :: ((i < k < a.Length) && c[j] == a[k] && j == position(key(a[k]), k, a[..]))) //every filled in element of c is a previously seen elt
   invariant(forall x : int :: filter(a[(i+1)..], y => key(y) == x) == filter(filter(c[..], y => y != default), y => key(y) == x)) 
   
   {
-/*
-  assume(-1 <= i < a.Length);
-  assume(b1.Length == b.Length); //need for bounds
-  assume(forall j :: 0 <= j < a.Length ==> 0 <= key(a[j]) < b1.Length); //also need for bounds
-  assume(forall j : int :: 0 <= j < b1.Length ==> b1[j] <= numLeq(j, a[..], key) - 1); //used for bounds checks
-  //technically, this invariant is implied by the next one (by permutation_length), but the proofs are much faster if we include both
-  assume(|filter(c[..], y => y != default)| == a.Length - (i + 1)); //ensures that we fill all of c
-  assume(permutation((a[(i+1)..]),(filter(c[..], y => y != default)))); //permutation invariant
-  assume(forall j :: 0 <= j < b.Length ==> b1[j] == position(j, i, a[..], key)); //the array b at each step (b is changing)
-  assume(forall j :: 0 <= j < c.Length ==> c[j] != default ==> exists k :: ((i < k < a.Length) && c[j] == a[k] && j == position(key(a[k]), k, a[..], key))); //every filled in element of c is a previously seen elt
-  assume(forall x : int :: filter(a[(i+1)..], y => key(y) == x) == filter(filter(c[..], y => y != default), y => key(y) == x));*/
     //make sure everything is in bounds
     assert(0 <= i < a.Length);
     var ai := key(a[i]);
     assert(0 <= ai < b1.Length);
     //first, show that b[a[i]] is nonnegative
-    numEq_in_pos(a[i], a[..(i+1)], key);
+    numEq_in_pos(a[i], a[..(i+1)]);
     assert(0 <= b1[ai]);
     //then, show that it is bounded
     //ghost var ai := key(a[i]);
     filter_length_leq(a[..], y => key(y) <= ai);
-    numLeq_direct(ai, a[..], key);
+    numLeq_direct(ai, a[..]);
     assert(0 <= b1[ai] < c.Length);
   
     //ghost variables to refer to the old values of variables
@@ -1136,9 +1130,9 @@ requires(key(default) < 0)
 
 
 
-    no_default_elts(a, default, key);  
+    no_default_elts(a, default);  
     //A crucial step: show that c[b1[a[i]]] == -1, so we are actually considering a new element
-    sortedArrayLoopSeesNewElt(a, b1, c, i, default, key);
+    sortedArrayLoopSeesNewElt(a, b1, c, i, default);
     assert(c[idx] == default);
   
    
@@ -1159,59 +1153,59 @@ requires(key(default) < 0)
 
     
     //re-establish invariants with auxilliary lemmas
-    permutation_invariant(a, c[..], oldC, idx, i, default, key);
+    permutation_invariant(a, c[..], oldC, idx, i, default);
     assert(permutation((a[i..]),(filter(c[..], y => y != default)))); 
-    filter_length_invariant(a, c[..], oldC, idx, i, default, key);
-    assert(forall j : int :: 0 <= j < |oldB| ==> oldB[j] <= numLeq(j, a[..], key) - 1);
+    filter_length_invariant(a, c[..], oldC, idx, i, default);
+    assert(forall j : int :: 0 <= j < |oldB| ==> oldB[j] <= numLeq(j, a[..]) - 1);
    
 
-    b_position_invariant(a, oldB, b1[..], i, idx, key);
-    assert((forall j :: 0 <= j < b.Length ==> b1[j] == position(j, i-1, a[..], key)));
-     b_bound_invariant(a, oldB, b1[..], i, idx, key);
+    b_position_invariant(a, oldB, b1[..], i, idx);
+    assert((forall j :: 0 <= j < b.Length ==> b1[j] == position(j, i-1, a[..])));
+     b_bound_invariant(a, oldB, b1[..], i, idx);
     assert(|oldC| == cLen);
    // assume(forall j :: 0 <= j < c.Length ==> c[j] != default ==> exists k :: ((i < k < a.Length) && c[j] == a[k] && j == position(key(a[k]), k, a[..], key))); //every filled in element of c is a previously seen elt   
    
-      assert(forall j :: 0 <= j < |oldC| ==> oldC[j] != default ==> exists k :: ((i < k < a.Length) && oldC[j] == a[k] && j == position(key(a[k]), k, a[..], key)));
+      assert(forall j :: 0 <= j < |oldC| ==> oldC[j] != default ==> exists k :: ((i < k < a.Length) && oldC[j] == a[k] && j == position(key(a[k]), k, a[..])));
 
-    c_structure_invariant(a, oldB, c[..], oldC, idx, i, default, key);   
-    assert (forall j :: 0 <= j < c.Length ==> c[j] != default ==> exists k :: ((i - 1 < k < a.Length) && c[j] == a[k] && j == position(key(a[k]), k, a[..], key))); 
+    c_structure_invariant(a, oldB, c[..], oldC, idx, i, default);   
+    assert (forall j :: 0 <= j < c.Length ==> c[j] != default ==> exists k :: ((i - 1 < k < a.Length) && c[j] == a[k] && j == position(key(a[k]), k, a[..]))); 
     assert(key(default) < 0);
-    stable_invariant_preserved(a, oldB, oldC, c[..], i, a[i], idx, default, key); 
+    stable_invariant_preserved(a, oldB, oldC, c[..], i, a[i], idx, default); 
     
     
     
     i := i - 1;
-    /*
-    //some of the proofs seem to go better if we tell Dafny that the invariant holds explicitly (TODO: see if we need this)
-    assert(permutation((a[(i+1)..]),(filter(c[..], y => y != default))));
-    assert((forall j :: 0 <= j < b.Length ==> b1[j] == position(j, i, a[..], key)));
-    //assert(forall j :: 0 <= j < c.Length ==> c[j] != default ==> exists k :: (i < k < a.Length) && c[j] == a[k]);
-    assert (forall j :: 0 <= j < c.Length ==> c[j] != default ==> exists k :: ((i < k < a.Length) && c[j] == a[k] && j == position(key(a[k]), k, a[..], key))); 
+    
+    // //some of the proofs seem to go better if we tell Dafny that the invariant holds explicitly (TODO: see if we need this)
+    // assert(permutation((a[(i+1)..]),(filter(c[..], y => y != default))));
+    // assert((forall j :: 0 <= j < b.Length ==> b1[j] == position(j, i, a[..], key)));
+    // //assert(forall j :: 0 <= j < c.Length ==> c[j] != default ==> exists k :: (i < k < a.Length) && c[j] == a[k]);
+    // assert (forall j :: 0 <= j < c.Length ==> c[j] != default ==> exists k :: ((i < k < a.Length) && c[j] == a[k] && j == position(key(a[k]), k, a[..], key))); 
 
-    assert(forall j :: 0 <= j < a.Length ==> 0 <= key(a[j]) < b1.Length); //also need for bounds
-    assert(forall j : int :: 0 <= j < b1.Length ==> b1[j] <= numLeq(j, a[..], key) - 1); //used for bounds checks
-    //technically, this invariant is implied by the next one (by permutation_length), but the proofs are much faster if we include both
-    assert(|filter(c[..], y => y != default)| == a.Length - (i + 1)); //ensures that we fill all of c
-    assert(forall x : int :: filter(a[(i+1)..], y => key(y) == x) == filter(filter(c[..], y => y != default), y => key(y) == x));
-    assert(-1 <= i < a.Length);
-    assert(b1.Length == b.Length); //need for bounds 
-    */
+    // assert(forall j :: 0 <= j < a.Length ==> 0 <= key(a[j]) < b1.Length); //also need for bounds
+    // assert(forall j : int :: 0 <= j < b1.Length ==> b1[j] <= numLeq(j, a[..], key) - 1); //used for bounds checks
+    // //technically, this invariant is implied by the next one (by permutation_length), but the proofs are much faster if we include both
+    // assert(|filter(c[..], y => y != default)| == a.Length - (i + 1)); //ensures that we fill all of c
+    // assert(forall x : int :: filter(a[(i+1)..], y => key(y) == x) == filter(filter(c[..], y => y != default), y => key(y) == x));
+    // assert(-1 <= i < a.Length);
+    // assert(b1.Length == b.Length); //need for bounds 
+    
   }
-  /*
+  
   //invariants => postcondition (do in different lemmas so it is faster)
-  afterLoopPermutation(a, c);
+  afterLoopPermutation(a, c, default);
   assert(permutation(a[..], c[..]));
-  afterLoopSorted(a, c);
+  afterLoopSorted(a, c, default);
   assert(sorted(c[..]));
-  afterLoopStable(a, c);
+  afterLoopStable(a, c, default);
   assert(stable(a[..], c[..])); 
-  assume(false);*/
 } 
-/*
+
 //The final algorithm
-method countingSort(a: array<int>, k : int) returns (s: array<int>)
+method countingSort(a: array<G>, k : int, default : G) returns (s: array<G>)
 requires(0 < k)
-requires (forall i: int :: 0 <= i < a.Length ==> 0 <= a[i] < k)
+requires (forall i: int :: 0 <= i < a.Length ==> 0 <= key(a[i]) < k)
+requires(key(default) < 0)
 ensures(sorted(s[..]))
 ensures(permutation(a[..], s[..]))
 ensures(stable(a[..], s[..]))
@@ -1222,6 +1216,6 @@ ensures(stable(a[..], s[..]))
   else {
     var b := countOccurrences(a, k);
     var c := prefixSum(a, b);
-    s := constructSortedArray(a, c);
+    s := constructSortedArray(a, c, default);
   }
-}*/
+}
